% ---------------------- setting ---------------------- %
\documentclass[10pt,landscape,a4paper]{article}
\input{../Math.tex}
\usepackage[margin=0.5in]{geometry}
\usepackage{multicol}
\usepackage{fancyhdr}
\usepackage{amsmath, amsfonts, mathtools, amsthm, amssymb, mathrsfs}

\setlength\parindent{0pt}

\setlength{\columnseprule}{0.5pt}
\pagestyle{fancy}
\renewcommand{\headrulewidth}{0pt}
\fancyhf{}
\fancyhead{}
\fancyfoot{}

\begin{document}
\begin{multicols}{4}
% ---------------------- Content ---------------------- %
\section*{Probability Functions}
\subsection*{PMF/PDF, CDF, Expected Value, Variance}
\subsubsection*{General} 
(*independent assumed)
\[
  \mathbb{E}[X] = \mu = \sum_{x} xp_X (x) = \int_{-\infty}^{\infty} xf_X(x)dx
\]
\[
  \mathbb{E}[\alpha X + \beta Y] = \alpha \mathbb{E}[X] + \beta \mathbb{E}[Y]
\]
\[
  *\mathbb{E}[XY] = \mathbb{E}[X]\mathbb{E}[Y]
\]
\[
  \Var[X] = \mathbb{E}\left[(X - \mu)^2 \right] = \mathbb{E}[X^2] - \mathbb{E}[X]^2
\]
\[
  *\Var[X + Y] = \Var[X] + \Var[Y]
\]
\[
  \sigma_X \coloneqq \sqrt{\Var[X]} =  \sqrt{\mathbb{E}\left[(X - \mu)^2 \right]} 
\]

\subsubsection*{\(X \sim \text{Bernoulli}(p)\)}
\[
  p_X (x) = \begin{dcases}
    1 - p &\text{ if } x = 0\\
    p &\text{ if } x = 1
  \end{dcases}
\]
\[
  \mathbb{E}[X] = p \quad\quad \Var[X] = p(1 - p)
\]

\subsubsection*{\(X \sim \text{Binomial}(n, p)\)}
\[
  p_X (k) = \mathbb{P}(X = k) = \binom{n}{k}p^k(1 - p)^{n-k}
\]
\[
  \mathbb{E}[X] = np \quad\quad \Var[X] = np(1 - p)
\]

\subsubsection*{\(X \sim \text{Geometric}(p)\)}
\[
  p_X (k) = \mathbb{P}(X = k) = p(1 - p)^{k-1} 
\]
\[
  \mathbb{E}[X] = \frac{1}{p} \quad\quad \Var[X] = \frac{1 - p}{p^{2}}
\]

\subsubsection*{\(X \sim \text{Poisson}(\lambda)\)}
\[
  p(k) = e^{-\lambda}\dfrac{\lambda^k}{k!}, \quad k = 0, 1, 2, 3
\]
\[
  \mathbb{E}[X] = \lambda \quad\quad \Var[X] = \lambda 
\]

\subsubsection*{\(X \sim \text{Uniform}(a, b)\)}
\[
    F_X(x) = \begin{dcases}
        0, &\text{ if } x < a \\
        \frac{x - a}{b - a}, &\text{ if } a \leq x \leq b \\
        1 , &\text{ if } b < x
    \end{dcases}
\]
\[
  f_X(x) = \begin{dcases}
    0, &\text{ if } x < a \\
    \frac{1}{b - a}, &\text{ if } a \leq x \leq b \\
    0 , &\text{ if } b < x
  \end{dcases}
\]
\[
  \mathbb{E}[X] = \dfrac{a + b}{2} \quad\quad \Var[X] = \dfrac{(b - a)^2}{12}
\]

\subsubsection*{\(X \sim \text{Exponential}(\lambda)\)}
\[
  f_X(x) = \begin{dcases}
    \lambda e^{-\lambda x} , &\text{ if }  x \geq 0\\
    0 , &\text{ if } x < 0
  \end{dcases}
\]
\[
    F_X(x) = 1 - e^{- \lambda x}
\]
\[
  \mathbb{E}[X] = \dfrac{1}{\lambda} \quad\quad \Var[X] = \dfrac{1}{\lambda^2}
\]

\subsection*{Joint PMF}
\[
    p(x, y) = \mathbb{P}(X = x, Y = y)
\]

\subsection*{Normal Distribution}
\(X \sim \mathcal{N}(\mu, \sigma^2)\) 
\[
  f_X(x) = \dfrac{1}{\sqrt{2\pi \sigma ^2}}e^{-\frac{(x - \mu)^2}{2\sigma^2}}
\]
\[
    \mathbb{E}[X] = \mu \quad\quad \Var[X] = \sigma^2
\]

\subsection*{Standard Normal Distribution}
\(\mathcal{N}(0, 1)\) 
\[
  f_X(x) \coloneqq \dfrac{1}{\sqrt{2\pi}} e^{-\frac{x^2}{2}}
\]
\[
  \mathbb{E}[Z] = 0 \quad\quad \Var[Z] = 1.
\]
Convert: 
\[
  Z = \frac{X - \mu}{\sigma}
\]

\subsection*{Central Limit Theorem}
\[
  Z_n = \dfrac{S_n - n\mu}{\sigma\sqrt{n}},\  S_n = X_1 + \cdots + X_n
\]
\[
  \lim_{n \to \infty} \mathbb{P}(Z_n \leq z) = \varPhi (z)
\]

\section*{Bayesian Statistic}
\subsection*{Bayes' rule}
\[
  \underbrace{f_{\Theta \vert X} (\theta \vert x)}_{\text{Posterior}} = \dfrac{\overbrace{f_{\Theta} (\theta)}^{\text{Prior}} \overbrace{f_{X \vert \Theta} (x \vert \theta)}^{\text{Observation}}}{f_X (x)}
\]
\[
  \underbrace{f_{\Theta \vert X} (\theta \vert x)}_{\text{posterior}} \propto \underbrace{f_{X \vert \Theta} (x \vert \theta)}_{\text{likelihood}} \underbrace{f_{\Theta} (\theta)}_{\text{prior}}
\]

\subsection*{Beta Distribution}
\[
  f_{\Theta} (\theta) = \begin{dcases}
    \underbrace{\dfrac{1}{B(\alpha, \beta)} \theta^{\alpha-1} (1 - \theta)^{\beta - 1}}_{\text{if}\ 0 < \theta < 1} \\
    0 \quad \text{ otherwise} 
  \end{dcases}
\]

\subsection*{Gamma Distribution}
\[
  f_{\Theta} (\theta) = \begin{dcases}
    \dfrac{\beta^{\alpha}}{\Gamma (\alpha)}\theta^{\alpha - 1} e^{-\beta\theta} &\text{ for } \theta > 0 \\
    0 &\text{ for } \theta \leq 0 \\
  \end{dcases}
\]

\vfill\break
% ---------------------- END ---------------------- %
\end{multicols}
\end{document}